updates

Veritas.Verifier.Merkle.fst
@@ -2547,12 +2547,16 @@ let lemma_proving_ancestor_has_hash (itsl: TL.eac_log) (k:key{k<> Root}):
                                   (desc_dir k (proving_ancestor itsl k)) =
                   hashfn (eac_value itsl k))) = lemma_proving_ancestor_has_hash_aux itsl k
 
+let is_in_blum (es: eac_state): bool = 
+  EACEvictedBlum? es || 
+  (EACInStore? es && EACInStore?.m es = BAdd)
+
 let proving_ancestor_has_blum_bit (itsl: TL.eac_log) (k:key {k <> Root}): bool = 
-  not (TL.is_eac_state_evicted itsl k) || 
+  let es = eac_state_of_key itsl k in
+  not (is_eac_state_active es) || 
   mv_evicted_to_blum (eac_merkle_value itsl (proving_ancestor itsl k))
                                      (desc_dir k (proving_ancestor itsl k)) =
-                  is_eac_state_evicted_blum itsl k
-
+                      is_in_blum es
 
 let lemma_proving_ancestor_has_blum_bit_extend_memop (itsl: TL.eac_log {I.length itsl > 0}) (k: key{k <> Root}):
   Lemma (requires (let n = I.length itsl in
@@ -2565,30 +2569,168 @@ let lemma_proving_ancestor_has_blum_bit_extend_memop (itsl: TL.eac_log {I.length
   let e = I.index itsl (n - 1) in
   
   let itsl' = I.prefix itsl (n - 1) in
+  let es = TL.eac_state_of_key itsl k in
   let es' = TL.eac_state_of_key itsl' k in
 
-  if not (TL.is_eac_state_evicted itsl k) then ()
-  else (
-    lemma_fullprefix_equal itsl;
+  lemma_fullprefix_equal itsl;
+  lemma_eac_state_of_key_valid itsl k;
+  lemma_eac_state_of_key_valid itsl' k;
+
+  if not (is_eac_state_active es) then ()
+  else if k = V.key_of e then (
     lemma_eac_state_transition itsl (n - 1);
-    lemma_eac_state_of_key_valid itsl' k;    
-    
-    lemma_eac_value_unchanged_memop itsl k;
-    // assert(eac_value itsl k = eac_value itsl' k);
-    
+    // assert(EACInStore? es);
+    // assert(EACInStore?.m es = EACInStore?.m es');
+    // assert(is_in_blum es = is_in_blum es');
+
+    (* proving ancestor is unchanged *)
     lemma_ptrfn_unchanged itsl;
-    // assert(feq_ptrfn (eac_ptrfn itsl) (eac_ptrfn itsl'));
-
-    (* proving ancestor is unchanged when processing e *)
     let pk = proving_ancestor itsl k in
-    lemma_feq_proving_ancestor (eac_ptrfn itsl) (eac_ptrfn itsl') k;    
+    lemma_feq_proving_ancestor (eac_ptrfn itsl) (eac_ptrfn itsl') k;
     // assert(pk = proving_ancestor itsl' k);
-
     
-    lemma_eac_value_unchanged_memop itsl pk;
-    // assert(eac_value itsl pk = eac_value itsl' pk);
+    lemma_eac_value_unchanged_memop itsl pk
+  )
+  else (
+    lemma_eac_state_same itsl (n - 1) k;
+    lemma_ptrfn_unchanged itsl;
+    let pk = proving_ancestor itsl k in
+    lemma_feq_proving_ancestor (eac_ptrfn itsl) (eac_ptrfn itsl') k;
+    // assert(pk = proving_ancestor itsl' k);
+    
+    lemma_eac_value_unchanged_memop itsl pk    
+  )
 
-    lemma_eac_state_same itsl (n - 1) k
+let lemma_proving_ancestor_has_blum_bit_extend_evictm (itsl: TL.eac_log {I.length itsl > 0}) (k: key{k <> Root}):
+  Lemma (requires (let n = I.length itsl in
+                   let e = I.index itsl (n - 1) in
+                   let itsl' = I.prefix itsl (n - 1) in
+                   proving_ancestor_has_blum_bit itsl' k /\
+                   (EvictM? e \/ EvictBM? e)))
+        (ensures (proving_ancestor_has_blum_bit itsl k)) = 
+  let n = I.length itsl in
+  let e = I.index itsl (n - 1) in
+  let tid = TL.thread_id_of itsl (n - 1) in
+  let vs = TL.thread_state itsl tid in
+  let pf = eac_ptrfn itsl in
+  let itsl' = I.prefix itsl (n - 1) in
+  let es = TL.eac_state_of_key itsl k in
+  let es' = TL.eac_state_of_key itsl' k in
+  let vs' = TL.thread_state itsl' tid in
+  let st' = TL.thread_store itsl' tid in  
+
+  if not (is_eac_state_active es) then ()
+  else (
+    match e with
+    | EvictM k1 k2 
+    | EvictBM k1 k2 _ ->
+
+      lemma_fullprefix_equal itsl;
+      lemma_verifier_thread_state_extend itsl (n - 1);  
+      lemma_eac_state_transition itsl (n - 1);
+      lemma_eac_state_of_key_valid itsl k;
+      lemma_eac_state_of_key_valid itsl' k;      
+
+      if k1 = k then (
+        let pk = proving_ancestor itsl k in
+        lemma_ptrfn_unchanged itsl;
+        lemma_feq_proving_ancestor (eac_ptrfn itsl) (eac_ptrfn itsl') k;
+        lemma_evict_ancestor_is_proving itsl;
+        //assert(pk = k2);
+        
+        lemma_eac_value_is_stored_value itsl pk tid        
+      )
+      else if k2 = k then (
+        lemma_instore_implies_eac_state_instore itsl k tid;
+        lemma_eac_state_same itsl (n - 1) k;
+
+        lemma_ptrfn_unchanged itsl;
+        let pk = proving_ancestor itsl k in
+        lemma_feq_proving_ancestor (eac_ptrfn itsl) (eac_ptrfn itsl') k;
+        assert(pk = proving_ancestor itsl' k);
+
+        lemma_eac_value_unchanged_evictm itsl pk
+      )
+      else (
+        lemma_eac_state_same itsl (n - 1) k;
+        assert(es = es');
+
+        lemma_ptrfn_unchanged itsl;
+        let pk = proving_ancestor itsl k in
+        lemma_feq_proving_ancestor pf (eac_ptrfn itsl') k;
+
+        (* pk is root reachable *)
+        // assert(BP.root_reachable pf pk);
+        lemma_eac_state_of_key_valid itsl pk;
+        lemma_not_init_equiv_root_reachable itsl pk;
+        // assert(pk = Root || TL.is_eac_state_active itsl pk);
+
+        if pk = k2 then (
+          lemma_evict_ancestor_is_proving itsl;
+          lemma_feq_proving_ancestor pf (eac_ptrfn itsl') k1;
+          // assert(pk = proving_ancestor itsl k1);
+          lemma_proving_ancestor_points_to_self itsl k;
+
+          lemma_eac_state_transition itsl (n - 1);
+          lemma_eac_state_of_key_valid itsl k1;
+          lemma_eac_state_of_key_valid itsl' k1;
+          // assert(TL.is_eac_state_evicted itsl k1);
+          lemma_proving_ancestor_points_to_self itsl k1;
+
+          // assert(desc_dir k pk = other_dir (desc_dir k1 pk));
+          lemma_eac_value_unchanged_evictm_anc_other_dir itsl
+        )
+        else
+          lemma_eac_value_unchanged_evictm itsl pk      
+      )
+  )
+
+
+let lemma_proving_ancestor_has_blum_bit_extend_evictb (itsl: TL.eac_log {I.length itsl > 0}) (k: key{k <> Root}):
+  Lemma (requires (let n = I.length itsl in
+                   let e = I.index itsl (n - 1) in
+                   let itsl' = I.prefix itsl (n - 1) in
+                   proving_ancestor_has_blum_bit itsl' k /\
+                   EvictB? e))
+        (ensures (proving_ancestor_has_blum_bit itsl k)) = 
+  let n = I.length itsl in
+  let e = I.index itsl (n - 1) in
+  let itsl' = I.prefix itsl (n - 1) in
+  let tid = TL.thread_id_of itsl (n - 1) in
+  let pf = eac_ptrfn itsl in
+  let es = TL.eac_state_of_key itsl k in
+  let es' = TL.eac_state_of_key itsl' k in
+  
+
+
+  if not (is_eac_state_active es) then ()
+  else (
+    match e with
+    | EvictB k1 _ ->
+
+      lemma_fullprefix_equal itsl;
+      lemma_verifier_thread_state_extend itsl (n - 1);
+      lemma_eac_state_transition itsl (n - 1);
+
+      if k1 = k then (
+        assert(is_in_blum es = is_in_blum es');
+        
+        let pk = proving_ancestor itsl k in
+        lemma_ptrfn_unchanged itsl;
+        lemma_feq_proving_ancestor (eac_ptrfn itsl) (eac_ptrfn itsl') k;
+        assert(pk = proving_ancestor itsl' k);
+
+        lemma_eac_value_unchanged_evictb itsl pk
+      )
+      else (
+        lemma_eac_state_same itsl (n - 1) k;
+        let pk = proving_ancestor itsl k in
+        lemma_ptrfn_unchanged itsl;
+        lemma_feq_proving_ancestor (eac_ptrfn itsl) (eac_ptrfn itsl') k;
+        assert(pk = proving_ancestor itsl' k);
+
+        lemma_eac_value_unchanged_evictb itsl pk
+      )
   )
 
 (* when evicted as blum the proving ancestor contains a bit indicating the eviction *)
@@ -2606,8 +2748,10 @@ let rec lemma_proving_ancestor_blum_bit_aux (itsl: TL.eac_log) (k:key{k <> Root}
     match e with
     | Get _ _ 
     | Put _ _ -> lemma_proving_ancestor_has_blum_bit_extend_memop itsl k
+    | EvictBM _ _ _ 
+    | EvictM _ _ -> lemma_proving_ancestor_has_blum_bit_extend_evictm itsl k
+    | EvictB _ _ -> lemma_proving_ancestor_has_blum_bit_extend_evictb itsl k
     | _ -> 
-
     admit()
   )
 
